pulse/lib/pulse/lib/pledge/Pulse.Lib.Trade.fsti
@@ -44,20 +44,20 @@ val intro_trade
     (fun _ -> invlist_v is ** concl)
   ))
 : stt_ghost unit emp_inames
-    extra
+    (invlist_inv is ** extra)
     (fun _ -> trade #is hyp concl)
 
 val elim_trade
   (#[T.exact (`invlist_empty)] is : invlist)
   (hyp concl: vprop)
 : stt_ghost unit (invlist_names is)
-    (invlist_inv is ** (trade #is hyp concl) ** hyp)
-    (fun _ -> invlist_inv is ** concl)
+    (trade #is hyp concl ** hyp)
+    (fun _ -> concl)
 
 val trade_sub_inv
   (#os1 : invlist)
   (#os2 : invlist{invlist_sub os1 os2})
   (hyp concl: vprop)
 : stt_ghost unit (invlist_names os1)
-    (invlist_inv os1 ** trade #os1 hyp concl)
-    (fun _ -> invlist_inv os1 ** trade #os2 hyp concl)
+    (invlist_inv os2 ** trade #os1 hyp concl)
+    (fun _ -> trade #os2 hyp concl)
